MiniKernel/Proofs.lean
@@ -1,0 +1,126 @@
+import MiniKernel.Kernel
+
+def Level.eval (l : Level) (ctx : Name → Nat) : Nat :=
+  match l with
+  | .zero => 0
+  | .succ l' => l'.eval ctx + 1
+  | .max l1 l2 => Nat.max (l1.eval ctx) (l2.eval ctx)
+  | .imax l1 l2 => if (l2.eval ctx) = 0 then 0 else Nat.max (l1.eval ctx) (l2.eval ctx)
+  | .param n => ctx n
+
+@[grind] inductive Level.NF : Level → Prop
+  | zero : Level.NF .zero
+  | succ : Level.NF l → Level.NF (.succ l)
+  | max : Level.NF l1 → Level.NF l2 → Level.NF (.max l1 l2)
+  | imax : Level.NF l1 → Level.NF (.imax l1 (.param u))
+  | param : Level.NF (.param n)
+
+@[grind .] theorem Level.NF.mkIMax (h1 : Level.NF l1) (h2 : Level.NF l2) : Level.NF (.mkIMax l1 l2) := by
+  fun_induction Level.mkIMax <;> grind
+
+@[grind .] theorem Level.NF.simplify : Level.NF (simplify l) := by
+  fun_induction Level.simplify <;> grind
+
+@[grind =] theorem Level.mkIMax_correct (ctx : Name → Nat) (l1 l2 : Level): (mkIMax l1 l2).eval ctx = (Level.imax l1 l2).eval ctx := by
+  fun_induction mkIMax<;> try grind [Level.eval]
+
+@[simp] theorem Level.elimIMax_correct (ctx : Name → Nat) (l : Level): l.elimIMax.eval ctx = l.eval ctx := by
+  fun_induction Level.elimIMax <;> grind [Level.eval]
+
+@[simp] theorem Level.simplify_correct (ctx : Name → Nat) (l : Level): l.simplify.eval ctx = l.eval ctx := by
+  fun_induction Level.simplify <;> grind [Level.eval]
+
+theorem Level.substOneLevel_eval' {ctx ctx' p} (l1 l2 : Level)
+  (h : l2.eval ctx' = ctx p)
+  (h2 : ∀ p', p ≠ p' → ctx' p' = ctx p') :
+  (l1.substOneLevel p l2).eval ctx' = l1.eval ctx := by
+  unfold substOneLevel
+  fun_induction substLevel <;> grind [Level.eval]
+
+theorem Level.substOneLevel_eval (l1 l2 : Level) (h : l2.eval ctx = ctx p):
+  (l1.substOneLevel p l2).eval ctx = l1.eval ctx :=
+  Level.substOneLevel_eval' _ _ h (by grind)
+
+theorem Level.le_correct (ctx : Name → Nat) (l1 l2 : Level) balance : l1.le l2 balance = true → l1.eval ctx ≤ l2.eval ctx + balance := by
+  fun_induction Level.le l1 l2 balance generalizing ctx <;> try grind [Level.eval]
+  case case6 l2 balance l1 p _ _ ih =>
+    match h : ctx p with
+    | .zero =>
+      unfold byCases
+      specialize ih ((l1.imax (param p)).substOneLevel p .zero).elimIMax
+                    (l2.substOneLevel p .zero).elimIMax
+                    (fun _ => by grind [countIMax, elimIMax])
+                    ctx
+      simp [elimIMax] at ih
+      intro hle
+      specialize ih (by simp [elimIMax] at hle; grind)
+      simp [eval] at ih
+      rw [Level.substOneLevel_eval] at ih
+      case h => simp [h, eval]
+      simp [eval, h]
+      assumption
+    | .succ n =>
+      unfold byCases
+      specialize ih ((l1.imax (param p)).substOneLevel p ((Level.param p).succ)).elimIMax
+                    (l2.substOneLevel p ((Level.param p).succ)).elimIMax
+                    (fun _ => by grind [countIMax, elimIMax])
+                    (fun p' => if p' = p then n else ctx p')
+      simp [elimIMax] at ih
+      intro hle
+      specialize ih (by simp [elimIMax] at hle; grind)
+      simp [eval] at ih
+      rw [Level.substOneLevel_eval' (ctx := ctx)] at ih
+      case h => simp [h, eval]
+      case h2 => grind
+      rw [Level.substOneLevel_eval' (ctx := ctx)] at ih
+      case h => simp [h, eval]
+      case h2 => grind
+      simp [eval, h]
+      assumption
+  case case7 l1 balance l2 p _ _ _ ih =>
+    match h : ctx p with
+    | .zero =>
+      unfold byCases
+      specialize ih (l1.substOneLevel p .zero).elimIMax
+                    ((l2.imax (param p)).substOneLevel p .zero).elimIMax
+                    (fun _ => by grind [countIMax, elimIMax])
+                    ctx
+      simp [elimIMax] at ih
+      intro hle
+      specialize ih (by simp [elimIMax] at hle; grind)
+      simp [eval] at ih
+      rw [Level.substOneLevel_eval] at ih
+      case h => simp [h, eval]
+      simp [eval, h]
+      assumption
+    | .succ n =>
+      unfold byCases
+      specialize ih (l1.substOneLevel p ((Level.param p).succ)).elimIMax
+                   ((l2.imax (param p)).substOneLevel p ((Level.param p).succ)).elimIMax
+                    (fun _ => by grind [countIMax, elimIMax])
+                    (fun p' => if p' = p then n else ctx p')
+      simp [elimIMax] at ih
+      intro hle
+      specialize ih (by simp [elimIMax] at hle; grind)
+      simp [eval] at ih
+      rw [Level.substOneLevel_eval' (ctx := ctx)] at ih
+      case h => simp [h, eval]
+      case h2 => grind
+      rw [Level.substOneLevel_eval' (ctx := ctx)] at ih
+      case h => simp [h, eval]
+      case h2 => grind
+      simp [eval, h]
+      assumption
+
+/-
+-- I’m currently not sure if this is actually true, due to case 4 and `(∀, … ∨ …)`
+theorem Level.le_complete (ctx : Name → Nat) (l1 l2 : Level) (balance : Int) :
+    (∀ ctx, l1.eval ctx ≤ l2.eval ctx + balance) → l1.le l2 balance = true := by
+  intro hle
+  fun_induction Level.le l1 l2 balance <;> try grind [Level.eval]
+  case case4 ih1 ih2 =>
+    simp only [Bool.or_eq_true]
+    simp [eval, Lean.Omega.Int.ofNat_max, ← Int.max_add_right] at hle
+    sorry
+  all_goals sorry
+-/
